src/new_goose_lang/ffi/grove_ffi/grove_ffi.v
@@ -21,6 +21,7 @@ Section grove.
   (* these are local instances on purpose, so that importing this files doesn't
   suddenly cause all FFI parameters to be inferred as the grove model *)
   (* FIXME: figure out which of these clients need to set *)
+  Set Printing Projections.
   Existing Instances grove_op grove_model grove_semantics grove_interp goose_groveGS goose_groveNodeGS.
   Local Coercion Var' (s:string) : expr := Var s.
 
@@ -61,26 +62,61 @@ Section grove.
     wp_apply wp_AcceptOp. by iApply "HΦ".
   Qed.
 
-Ltac inv_undefined :=
-  match goal with
-  | [ H: relation.denote (match ?e with | _ => _ end) _ _ _ |- _ ] =>
-    destruct e; try (apply suchThat_false in H; contradiction)
-  end.
+  Ltac inv_undefined :=
+    match goal with
+    | [ H: relation.denote (match ?e with | _ => _ end) _ _ _ |- _ ] =>
+        destruct e; try (apply suchThat_false in H; contradiction)
+    end.
 
-Local Ltac solve_atomic :=
-  apply strongly_atomic_atomic, ectx_language_atomic;
-  [ apply heap_base_atomic; cbn [relation.denote base_trans]; intros * H;
-    repeat inv_undefined;
-    try solve [ apply atomically_is_val in H; auto ]
-    |apply ectxi_language_sub_redexes_are_values; intros [] **; naive_solver].
-Local Ltac solve_atomic2 :=
-  solve_atomic;
-  (* TODO(Joe): Cleanup *)
-  repeat match goal with
-    | [ H: relation.denote _ ?s1 ?s2 ?v |- _ ] => inversion_clear H
-    | _ => progress monad_inv
-    | _ => case_match
-    end; eauto.
+  Local Ltac solve_atomic :=
+    apply strongly_atomic_atomic, ectx_language_atomic;
+                                  [ apply heap_base_atomic; cbn [relation.denote base_trans]; intros * H;
+                                    repeat inv_undefined;
+                                    try solve [ apply atomically_is_val in H; auto ]
+                                  |apply ectxi_language_sub_redexes_are_values; intros [] **; naive_solver].
+  Local Ltac solve_atomic2 :=
+    solve_atomic;
+    (* TODO(Joe): Cleanup *)
+    repeat match goal with
+           | [ H: relation.denote _ ?s1 ?s2 ?v |- _ ] => inversion_clear H
+           | _ => progress monad_inv
+           | _ => case_match
+           end; eauto.
+
+  Local Lemma own_slice_to_pointsto_vals s q vs :
+    own_slice s byteT q vs -∗ pointsto_vals s.(slice.ptr_f) q vs.
+  Proof.
+    rewrite own_slice_unseal /own_slice_def /pointsto_vals.
+    iIntros "(Hs & _ & _)". simpl.
+    iApply (big_sepL_impl with "Hs").
+    iModIntro. iIntros "* % Hp". rewrite go_type_size_unseal /= left_id.
+    rewrite typed_pointsto_unseal /typed_pointsto_def.
+    iDestruct select (_) as "[Hp %Hty]". inversion Hty; subst.
+    simpl. rewrite right_id. rewrite loc_add_0. iFrame.
+  Qed.
+
+  Local Lemma pointsto_vals_to_own_slice p cap q d :
+    (length d) = uint.nat (length d) →
+    (length d) ≤ uint.Z cap →
+    pointsto_vals p q (data_vals d)-∗
+    own_slice (slice.mk p (length d) cap) byteT q (data_vals d).
+  Proof.
+    intros Hoverflow Hcap.
+    rewrite own_slice_unseal /own_slice_def /pointsto_vals.
+    iIntros "Hl". simpl.
+    iSplitL.
+    2:{ iPureIntro. rewrite /data_vals fmap_length /=. word. }
+    iApply (big_sepL_impl with "[$]").
+    iModIntro. iIntros "* % Hp". rewrite go_type_size_unseal /= left_id.
+    rewrite typed_pointsto_unseal /typed_pointsto_def.
+    rewrite /data_vals list_lookup_fmap /= in H.
+    destruct (d !! k).
+    2:{ exfalso. done. }
+    simpl in *. inversion H; subst.
+    iSplitL.
+    2:{ iPureIntro. econstructor. }
+    simpl. rewrite right_id. rewrite loc_add_0. iFrame.
+  Qed.
 
   Lemma wp_Send c_l c_r (s : slice.t) (data : list u8) (q : dfrac) :
     ⊢ {{{ own_slice s byteT q (data_vals data) }}}
@@ -95,22 +131,25 @@ Local Ltac solve_atomic2 :=
     iIntros "!#" (Φ) "Hs HΦ". wp_lam. wp_let.
     destruct s.
     wp_pures.
-    wp_apply wp_slice_ptr.
-    wp_apply wp_slice_len.
-    wp_pures.
-    iDestruct (own_slice_small_sz with "Hs") as "%Hlen".
-    iDestruct (own_slice_small_wf with "Hs") as "%Hwf".
+    iDestruct (own_slice_sz with "Hs") as "%Hlen".
+    iDestruct (own_slice_wf with "Hs") as "%Hwf".
     rewrite difference_empty_L.
     iMod "HΦ" as (ms) "[Hc HΦ]".
     { solve_atomic2. }
-    wp_apply (wp_SendOp with "[$Hc Hs]"); [done..| |].
-    { iApply own_slice_small_byte_pointsto_vals. done. }
+    cbn in *.
+    rewrite /data_vals fmap_length in Hlen.
+    wp_apply (wp_SendOp with "[$Hc Hs]").
+    { done. }
+    { iApply (own_slice_to_pointsto_vals with "[$]"). }
     iIntros (err_early err_late) "[Hc Hl]".
     iApply ("HΦ" $! (negb err_early) with "[Hc]").
     { by destruct err_early. }
     iSplit.
     - iPureIntro. by destruct err_early, err_late.
-    - iApply pointsto_vals_own_slice_small_byte; done.
+    - iDestruct (pointsto_vals_to_own_slice with "Hl") as "H".
+      { word. }
+      2:{ iExactEq "H". repeat f_equal. word. }
+      word.
   Qed.
 
   Lemma wp_Receive c_l c_r :
@@ -119,12 +158,12 @@ Local Ltac solve_atomic2 :=
       <<< ∃∃ (err : bool) (data : list u8),
         c_l c↦ ms ∗ if err then True else ⌜Message c_r data ∈ ms⌝
       >>>
-      {{{ (s : Slice.t),
-        RET struct.mk_f ReceiveRet [
+      {{{ (s : slice.t),
+        RET struct.val ReceiveRet [
               "Err" ::= #err;
-              "Data" ::= slice_val s
+              "Data" ::= slice.val s
             ];
-          own_slice s byteT (DfracOwn 1) data
+          own_slice s byteT (DfracOwn 1) (data_vals data)
       }}}.
   Proof.
     iIntros "!#" (Φ) "HΦ". wp_call. wp_pures.
@@ -138,15 +177,15 @@ Local Ltac solve_atomic2 :=
     { iFrame. destruct err; first done. iPureIntro. apply Hm. }
     iModIntro. wp_pures. iModIntro.
     destruct err.
-    { iApply ("HΦ" $! (Slice.mk _ _ _)). simpl. destruct Hm as (-> & -> & ->).
-      iApply own_slice_zero. }
+    { iApply ("HΦ" $! (slice.mk _ _ _)). simpl. destruct Hm as (-> & -> & ->).
+      simpl.
+      iApply own_slice_empty. done. }
     destruct Hm as [Hin Hlen].
-    iApply ("HΦ" $! (Slice.mk _ _ _)).
-    rewrite /own_slice.
-    iSplitL.
-    - iApply pointsto_vals_own_slice_small_byte; done.
-    - iExists []. simpl. iSplit; first by eauto with lia.
-      iApply array.array_nil. done.
+    iApply ("HΦ" $! (slice.mk _ _ _)).
+    iDestruct (pointsto_vals_to_own_slice with "Hl") as "H".
+    { word. }
+    2:{ iExactEq "H". repeat f_equal. word. }
+    word.
   Qed.
 
   Lemma wp_GetTSC :
